\documentclass{article}
\usepackage{amsmath,enumerate}
\title{CLRS 4-7}
\author{Peter Danenberg}
\DeclareMathOperator{\monge}{Monge}
\begin{document}
\maketitle

\begin{enumerate}[a.]
  \item
    \begin{enumerate}[i.]
    \item That $\monge(A_{m,n}) \to \forall 1\leq i< m,1\leq j <
      n(a_{i,j}+a_{i+1,j+1}\leq a_{i,j+1} + a_{i+1,j})$ follows
      directly from the definition of a monge array.
    \item 
      \begin{description}
      \item[Basis]
        \[a_{0,0}+a_{1,1}\leq a_{0,1}+a_{1,0}\to
        \monge(A_{2,2})\]
      \item[Hypothesis]
        \[\forall 1\leq i< m,1\leq j <
        n(a_{i,j}+a_{i+1,j+1}\leq a_{i,j+1} + a_{i+1,j}) \to
        \monge(A_{m,n})\]
      \item[Induction]
        \begin{align}
          \begin{split}
            \forall 1\leq i < m,1\leq j < n(a_{i,j}+a_{i+1,j+1}\leq
            a_{i,j+1} + a_{i+1,j}) &\to\\
            \forall j < n (a_{m,j} + a_{m+1,j+1} \leq a_{m,j+1} + a_{m+1,j}) \wedge\\
            \monge(A_{m,n})
          \end{split}\\
          &\to \monge(A_{m+1,n})
        \end{align}
        Similarly for $A_{m,n+1}$.
      \end{description}
    \end{enumerate}
    \item Changing either $a$ or $b$ to the given range will work.
      \[\begin{bmatrix}
        37&23&22&32\\
        21&6&7&10\\
        53&34&30&31\\
        43&21&15&8
      \end{bmatrix}
      \Rightarrow
      \begin{bmatrix}
        37&23&a\geq23&32\\
        21&6&b\leq6&10\\
        53&34&30&31\\
        43&21&15&8
      \end{bmatrix}\]
    \item $f(k) > f(k+1)$ violates the Monge definition by creating a
      minimum sum that no other combination of elements can undersum.

      Let $f(k) > f(k+1)$; pick $1 \leq q < r < m$ such that:
      \[\forall q \leq i < r, q < j \leq r (a_{k,i} > a_{k,r} \wedge a_{k+1,j} > a_{k+1, q})\]
      It follows, then, that
      \[\forall q \leq i < r, q < j \leq r (a_{k,i} + a_{k+1,j} > a_{k,r} + a_{k+1,q})\]
      contradicting the Monge definition.
    \item For each odd row $i$, start at column $j = f(i-1)$, where $f(0)
      = 0$; let $m_i = \infty$; iterate to $j = f(i+1)$, where $f(n+1)=m$;
      setting $m_i$ to $\min(m_i, a_{i,j})$.

      Running time is:
      \begin{align}
        \begin{split}
          O(m) + \sum_{i=1}^mf(i - 1)- f(i+1) &= O(m) + f(0) + f(m) + \\
          \sum_{i=1}^mf(i)-f(i)
        \end{split}\\
        &= O(m) + O(n) + 0\\
        &= O(m + n)
      \end{align}
    \item
      \begin{align}
        T(m) &= T(m/2) + O(m + n)\\
        &= \sum_{i=0}^{\lg m}2^i+n\\
        &= \Theta(m + n\lg m)
      \end{align}
\end{enumerate}
\end{document}
