\documentclass{article}
\usepackage{amsmath,clrscode}
\title{CLRS 15.2-4}
\author{Peter Danenberg}
\begin{document}
\maketitle

Since in \proc{Matrix-Chain-Order} the $i$-loop runs $n - l + 1$ times
for every $l$; and, for every $i$, the $k$-loop runs $j - i = i + l -
1 - i = j - l$ times; and, for every $k$, two $m[i,j]$s are looked up;
it gelds the following:

\begin{align}
  \sum_{i=1}^n\sum_{j=i}^n &= \sum_{l=2}^n2(n-l+1)(l-1)\\
  &= 2\sum_{l=1}^{n-1}(n-l)l\\
  &= 2\sum_{l=1}^{n-1}nl-2\sum_{l=1}^{n-1}l^2\\
  &= \frac{2n(n-1)n}{2} - \frac{2(n-1)n(2n-1)}{6}\\
  &= \frac{n^3 - n}{3}
\end{align}
\end{document}
